extraction: Some progress extracting the process scheduler

src/CertifiedExtraction/ADTExamples.v
@@ -1,3 +1,5 @@
+Require Import Fiat.Examples.QueryStructure.ProcessScheduler.
+
 Require Import
         CertifiedExtraction.Core
         CertifiedExtraction.FacadeUtils
@@ -6,16 +8,14 @@ Require Import
         CertifiedExtraction.Extraction.AllInternal
         CertifiedExtraction.Extraction.Extraction.
 
-Require Import Fiat.Examples.QueryStructure.ProcessScheduler.
-
 Definition MyEnvLists `{FacadeWrapper av (list W)} : Env av :=
-  (GLabelMap.add ("std", "rand") (Axiomatic FRandom))
-    ((GLabelMap.add ("list", "nil") (Axiomatic (FacadeImplementationOfConstructor nil)))
-       ((GLabelMap.add ("list", "push") (Axiomatic (FacadeImplementationOfMutation cons)))
-          ((GLabelMap.add ("list", "pop") (Axiomatic List_pop))
-             ((GLabelMap.add ("list", "delete") (Axiomatic (FacadeImplementationOfDestructor)))
-                ((GLabelMap.add ("list", "empty?") (Axiomatic List_empty))
-                   (GLabelMap.empty (FuncSpec _))))))).
+  (GLabelMap.empty (FuncSpec _))
+    ### ("std", "rand") ->> (Axiomatic FRandom)
+    ### ("list", "nil") ->> (Axiomatic (FacadeImplementationOfConstructor (list W) nil))
+    ### ("list", "push") ->> (Axiomatic (FacadeImplementationOfMutation_SCA (list W) cons))
+    ### ("list", "pop") ->> (Axiomatic (List_pop W))
+    ### ("list", "delete") ->> (Axiomatic (FacadeImplementationOfDestructor (list W)))
+    ### ("list", "empty?") ->> (Axiomatic (List_empty W)).
 
 Example other_test_with_adt'' `{FacadeWrapper av (list W)}:
     sigT (fun prog => forall seq: list W, {{ [[`"arg1" <-- seq as _ ]] :: Nil }}
@@ -32,10 +32,9 @@ Print Assumptions other_test_with_adt''. (* FIXME *)
 
 Opaque Word.wordToNat.
 Opaque Word.natToWord.
+Opaque nat_as_constant nat_as_word string_as_var.
 
 Eval compute in (extract_facade other_test_with_adt'').
-
-Eval cbv beta iota zeta delta [extract_facade Fold proj1_sig sig_of_sigT other_test_with_adt'' WrapOpInExpr] in (extract_facade other_test_with_adt'').
 
 Definition fold_comp {TAcc TElem} (f: Comp TAcc -> TElem -> Comp TAcc) seq init :=
   List.fold_left (fun (acc: Comp TAcc) (elem: TElem) =>
@@ -51,30 +50,19 @@ Require Import
 
 (* Opaque WrapInstance.            (* FIXME simpl never? *) *)
 
+Require Import FacadeLoops.
+
 Lemma CompileLoop :
-  forall `{FacadeWrapper av (list W)}
-    lst init vhead vtest vlst vret fpop fempty fdealloc facadeInit facadeBody env (ext: StringMap.t (Value av)) tenv (f: Comp W -> W -> Comp W),
-    GLabelMap.MapsTo fpop (Axiomatic List_pop) env ->
-    GLabelMap.MapsTo fempty (Axiomatic List_empty) env ->
-    GLabelMap.MapsTo fdealloc (Axiomatic (FacadeImplementationOfDestructor (A := list W))) env ->
-    vtest ∉ ext ->
-    NotInTelescope vtest tenv ->
-    vlst ∉ ext ->
-    NotInTelescope vlst tenv ->
-    vret ∉ ext ->
-    NotInTelescope vret tenv ->
-    vhead ∉ ext ->
-    NotInTelescope vhead tenv ->
-    vtest <> vret ->
-    vtest <> vlst ->
-    vtest <> vhead ->
-    vret <> vlst ->
-    vret <> vhead ->
-    vlst <> vhead ->
+  forall `{FacadeWrapper (Value av) A} `{FacadeWrapper (Value av) A'} `{FacadeWrapper av (list A)}
+    lst init vhead vtest vlst vret fpop fempty fdealloc facadeInit facadeBody env (ext: StringMap.t (Value av)) tenv (f: Comp A' -> A -> Comp A'),
+    GLabelMap.MapsTo fpop (Axiomatic (List_pop A)) env ->
+    GLabelMap.MapsTo fempty (Axiomatic (List_empty A)) env ->
+    GLabelMap.MapsTo fdealloc (Axiomatic (FacadeImplementationOfDestructor (list A))) env ->
+    PreconditionSet tenv ext [[[vhead; vtest; vlst; vret]]] ->
     {{ [[`vlst <~~ lst as _]] :: tenv }}
       facadeInit
     {{ [[`vret <~~ init as _]] :: [[`vlst <~~ lst as _]] :: tenv }} ∪ {{ ext }} // env ->
-    (forall head (acc: Comp W) (s: Comp (list W)),
+    (forall head (acc: Comp A') (s: Comp (list A)),
         {{ [[`vhead <-- head as _]] :: [[`vlst <~~ s as _]] :: [[`vtest <-- (bool2w false) as _]] :: [[`vret <~~ acc as _]] :: tenv }}
           facadeBody
         {{ [[`vlst <~~ s as _]] :: [[`vtest <-- (bool2w false) as _]] :: [[`vret <~~ (f acc head) as _]] :: tenv }} ∪ {{ ext }} // env) ->
@@ -82,7 +70,6 @@ Lemma CompileLoop :
       (Seq facadeInit (Seq (Fold vhead vtest vlst fpop fempty facadeBody) (Call vtest fdealloc (vlst :: nil))))
     {{ [[lst as ls]] :: [[`vret <~~ (fold_comp f ls init) as _]] :: tenv }} ∪ {{ ext }} // env.
 Proof.
-  Require Import FacadeLoops.
   loop_t.
 
   rewrite TelEq_swap by loop_t;
@@ -90,7 +77,7 @@ Proof.
 
   2:eapply CompileCallFacadeImplementationOfDestructor; loop_t.
 
-  rewrite (TelEq_swap _ NTNone) by loop_t.
+  rewrite (TelEq_swap _ NTNone).
 
   apply miniChomp'; loop_t.
 
@@ -99,75 +86,13 @@ Proof.
   generalize dependent lst;
   induction vv; loop_t.
 
-  rewrite TelEq_swap by loop_t.
+  rewrite TelEq_swap.
 
   apply CompileWhileFalse_Loop; loop_t.
 
   eapply CompileWhileTrue; loop_t.
 
-  apply generalized CompileCallPop; loop_t.
-
-  apply CompileCallEmpty_spec; loop_t.
-
-  loop_t.
-Qed.
-
-Lemma CompileLoop' :
-  forall {A} `{FacadeWrapper av (list W)} `{FacadeWrapper av A}
-    (lst: Comp (list W)) init vhead vtest vlst vret fpop fempty fdealloc facadeInit facadeBody env (ext: StringMap.t (Value av)) tenv (f: Comp A -> W -> Comp A),
-    GLabelMap.MapsTo fpop (Axiomatic List_pop) env ->
-    GLabelMap.MapsTo fempty (Axiomatic List_empty) env ->
-    GLabelMap.MapsTo fdealloc (Axiomatic (FacadeImplementationOfDestructor (A := list W))) env ->
-    vtest ∉ ext ->
-    NotInTelescope vtest tenv ->
-    vlst ∉ ext ->
-    NotInTelescope vlst tenv ->
-    vret ∉ ext ->
-    NotInTelescope vret tenv ->
-    vhead ∉ ext ->
-    NotInTelescope vhead tenv ->
-    vtest <> vret ->
-    vtest <> vlst ->
-    vtest <> vhead ->
-    vret <> vlst ->
-    vret <> vhead ->
-    vlst <> vhead ->
-    {{ [[`vlst <~~ lst as _]] :: tenv }}
-      facadeInit
-    {{ [[`vret <~~ init as _]] :: [[`vlst <~~ lst as _]] :: tenv }} ∪ {{ ext }} // env ->
-    (forall head (acc: Comp A) (s: Comp (list W)),
-        {{ [[`vhead <-- head as _]] :: [[`vlst <~~ s as _]] :: [[`vtest <-- (bool2w false) as _]] :: [[`vret <~~ acc as _]] :: tenv }}
-          facadeBody
-        {{ [[`vlst <~~ s as _]] :: [[`vtest <-- (bool2w false) as _]] :: [[`vret <~~ (f acc head) as _]] :: tenv }} ∪ {{ ext }} // env) ->
-    {{ [[`vlst <~~ lst as _]] :: tenv }}
-      (Seq facadeInit (Seq (Fold vhead vtest vlst fpop fempty facadeBody) (Call vtest fdealloc (vlst :: nil))))
-    {{ [[lst as ls]] :: [[`vret <~~ (fold_comp f ls init) as _]] :: tenv }} ∪ {{ ext }} // env.
-Proof.
-  loop_t.
-
-  rewrite TelEq_swap by loop_t;
-    eapply CompileCallEmpty_spec; loop_t.
-
-  2:eapply (CompileCallFacadeImplementationOfDestructor (A := list W)); loop_t.
-
-  loop_unify_with_nil_t.
-  
-  rewrite (TelEq_swap _ NTNone) by loop_t.
-
-  apply miniChomp'; loop_t.
-
-  clear dependent facadeInit;
-  generalize dependent init;
-  generalize dependent lst;
-  induction vv; loop_t.
-
-  rewrite TelEq_swap by loop_t.
-
-  apply CompileWhileFalse_Loop; loop_t.
-
-  eapply CompileWhileTrue; loop_t.
-
-  apply generalized CompileCallPop; loop_t.
+  apply generalized @CompileCallPop; loop_t.
 
   apply CompileCallEmpty_spec; loop_t.
 
@@ -175,33 +100,20 @@ Proof.
 Qed.
 
 Lemma CompileLoop_strong :
-  forall `{FacadeWrapper av (list W)}
+  forall `{FacadeWrapper (Value av) A} `{FacadeWrapper (Value av) A'} `{FacadeWrapper av (list A)}
     lst init vhead vtest vlst vret fpop fempty fdealloc facadeInit facadeBody facadeConclude
-    env (ext: StringMap.t (Value av)) tenv tenv' (f: Comp W -> W -> Comp W),
-    GLabelMap.MapsTo fpop (Axiomatic List_pop) env ->
-    GLabelMap.MapsTo fempty (Axiomatic List_empty) env ->
-    GLabelMap.MapsTo fdealloc (Axiomatic (FacadeImplementationOfDestructor (A := list W))) env ->
-    vtest ∉ ext ->
-    NotInTelescope vtest tenv ->
-    vlst ∉ ext ->
-    NotInTelescope vlst tenv ->
-    vret ∉ ext ->
-    NotInTelescope vret tenv ->
-    vhead ∉ ext ->
-    NotInTelescope vhead tenv ->
-    vtest <> vret ->
-    vtest <> vlst ->
-    vtest <> vhead ->
-    vret <> vlst ->
-    vret <> vhead ->
-    vlst <> vhead ->
+    env (ext: StringMap.t (Value av)) tenv tenv' (f: Comp A' -> A -> Comp A'),
+    GLabelMap.MapsTo fpop (Axiomatic (List_pop A)) env ->
+    GLabelMap.MapsTo fempty (Axiomatic (List_empty A)) env ->
+    GLabelMap.MapsTo fdealloc (Axiomatic (FacadeImplementationOfDestructor (list A))) env ->
+    PreconditionSet tenv ext [[[vhead; vtest; vlst; vret]]] ->
     {{ [[`vlst <~~ lst as _]] :: tenv }}
       facadeInit
     {{ [[`vret <~~ init as _]] :: [[`vlst <~~ lst as _]] :: tenv }} ∪ {{ ext }} // env ->
     {{ [[lst as ls]] :: [[`vret <~~ (fold_comp f ls init) as _]] :: tenv }}
       facadeConclude
     {{ [[lst as ls]] :: [[`vret <~~ (fold_comp f ls init) as _]] :: tenv' }} ∪ {{ ext }} // env ->
-    (forall head (acc: Comp W) (s: Comp (list W)),
+    (forall head (acc: Comp A') (s: Comp (list A)),
         {{ [[`vhead <-- head as _]] :: [[`vlst <~~ s as _]] :: [[`vtest <-- (bool2w false) as _]] :: [[`vret <~~ acc as _]] :: tenv }}
           facadeBody
         {{ [[`vlst <~~ s as _]] :: [[`vtest <-- (bool2w false) as _]] :: [[`vret <~~ (f acc head) as _]] :: tenv }} ∪ {{ ext }} // env) ->
@@ -220,15 +132,15 @@ Parameter TAcc : Type.
 Definition av := (list W + TSearchTerm + TAcc)%type.
 
 Definition MyEnvListsB : Env (list W + TSearchTerm + TAcc) :=
-  (GLabelMap.add ("std", "rand") (Axiomatic FRandom))
-    ((GLabelMap.add ("list", "nil") (Axiomatic (FacadeImplementationOfConstructor (@nil W))))
-       ((GLabelMap.add ("list", "push!") (Axiomatic (FacadeImplementationOfMutation (@cons W))))
-          ((GLabelMap.add ("list", "pop!") (Axiomatic List_pop))
-             ((GLabelMap.add ("list", "delete!") (Axiomatic (FacadeImplementationOfDestructor (A := list W))))
-                ((GLabelMap.add ("list", "empty?") (Axiomatic List_empty))
-                   ((GLabelMap.add ("search", "delete!") (Axiomatic (FacadeImplementationOfDestructor (A := TSearchTerm))))
-                      ((GLabelMap.add ("acc", "delete!") (Axiomatic (FacadeImplementationOfDestructor (A := TAcc))))
-                         (GLabelMap.empty (FuncSpec _))))))))).
+  (GLabelMap.empty (FuncSpec _))
+    ### ("std", "rand") ->> (Axiomatic FRandom)
+    ### ("listW", "nil") ->> (Axiomatic (FacadeImplementationOfConstructor (list W) nil))
+    ### ("listW", "push!") ->> (Axiomatic (FacadeImplementationOfMutation_SCA (list W) cons))
+    ### ("listW", "pop!") ->> (Axiomatic (List_pop W))
+    ### ("listW", "delete!") ->> (Axiomatic (FacadeImplementationOfDestructor (list W)))
+    ### ("listW", "empty?") ->> (Axiomatic (List_empty W))
+    ### ("search", "delete!") ->> (Axiomatic (FacadeImplementationOfDestructor TSearchTerm))
+    ### ("acc", "delete!") ->> (Axiomatic (FacadeImplementationOfDestructor TAcc)).
 
 Example other_test_with_adt''':
   sigT (fun prog => forall (searchTerm: TSearchTerm) (init: TAcc),
@@ -252,12 +164,12 @@ Proof.
 
   let av := av_from_ext (StringMap.empty (Value av)) in
   let fpop := find_function_pattern_in_env
-               (fun w => (Axiomatic (List_pop (av := av) (H := w)))) MyEnvListsB in
+               (fun w => (Axiomatic (List_pop (av := av) _ (H := w)))) MyEnvListsB in
   let fempty := find_function_pattern_in_env
-                 (fun w => (Axiomatic (List_empty (av := av) (H := w)))) MyEnvListsB in
+                 (fun w => (Axiomatic (List_empty (av := av) _ (H := w)))) MyEnvListsB in
   let fdealloc := find_function_pattern_in_env
                    (fun w => (Axiomatic (FacadeImplementationOfDestructor
-                                        (A := list W) (av := av) (H := w)))) MyEnvListsB in
+                                        (list W) (av := av) (H := w)))) MyEnvListsB in
   let vtest := gensym "test" in
   let vhead := gensym "head" in
   apply (CompileLoop_strong (vtest := vtest) (vhead := vhead) (fpop := fpop) (fempty := fempty) (fdealloc := fdealloc));
@@ -269,18 +181,20 @@ Proof.
   eapply CompileSeq.
   let fdealloc := find_function_pattern_in_env
                    (fun w => (Axiomatic (FacadeImplementationOfDestructor
-                                        (A := TSearchTerm) (av := av) (H := w)))) MyEnvListsB in
+                                        TSearchTerm (av := av) (H := w)))) MyEnvListsB in
   let vtmp := gensym "tmp" in
   apply (CompileCallFacadeImplementationOfDestructor (fpointer := fdealloc) (vtmp := vtmp));
     try compile_do_side_conditions.
 
   let fdealloc := find_function_pattern_in_env
                    (fun w => (Axiomatic (FacadeImplementationOfDestructor
-                                        (A := TAcc) (av := av) (H := w)))) MyEnvListsB in
+                                        TAcc (av := av) (H := w)))) MyEnvListsB in
   let vtmp := gensym "tmp" in
   apply (CompileCallFacadeImplementationOfDestructor (fpointer := fdealloc) (vtmp := vtmp));
     try compile_do_side_conditions.
 
+  compile_step.
+  apply CompileDeallocSCA_discretely. (* FIXME compile_do_extend_scalar_lifetime should consider Word.word 32 *)
   compile_step.
   compile_step.
   compile_step.
@@ -300,6 +214,246 @@ Defined.
 
 Eval compute in (extract_facade other_test_with_adt''').
 
+Definition revmap {A B} f := fun seq => @map A B f (rev seq).
+
+Lemma CompileMap_helper:
+  forall (A A' : Type) (f : A -> A') (a : A) (vv : list A) (base : list A'),
+    revmap f (a :: vv) ++ base = revmap f vv ++ f a :: base.
+Proof.
+  unfold revmap; intros; simpl.
+  rewrite map_rev.
+  rewrite map_app.
+  simpl.
+  rewrite <- app_assoc.
+  simpl.
+  rewrite <- map_rev.
+  reflexivity.
+Qed.
+
+Ltac defunctionalize_evar :=
+  match goal with
+  | [  |- context[?e] ] =>
+    is_evar e;
+      match type of e with
+      | ?a -> ?b => let ee := fresh in
+                  evar (ee: b);
+                    unify e (fun _:a => ee);
+                    unfold ee in *;
+                    clear ee
+      end
+  end.
+
+Ltac move_to_front var :=
+  repeat lazymatch goal with
+    | [  |- context[Cons ?k _ (fun _ => Cons (@NTSome _ _ var _) _ _)] ] =>
+      setoid_rewrite (TelEq_swap k (@NTSome _ _ var _)) at 1
+    end.
+
+Lemma CompileMap_ADT :
+  forall {av A A'} `{FacadeWrapper av (list A)} `{FacadeWrapper av (list A')} `{FacadeWrapper av A} `{FacadeWrapper av A'}
+    (base: list A') (lst: Comp (list A)) vhead vhead' vtest vlst vret vtmp fpop fempty falloc fdealloc fcons facadeBody env (ext: StringMap.t (Value av)) (tenv: Telescope av) (f: A -> A'),
+    GLabelMap.MapsTo fpop (Axiomatic (List_pop A)) env ->
+    GLabelMap.MapsTo fempty (Axiomatic (List_empty A)) env ->
+    GLabelMap.MapsTo falloc (Axiomatic (FacadeImplementationOfConstructor (list A') base)) env ->
+    GLabelMap.MapsTo fdealloc (Axiomatic (FacadeImplementationOfDestructor (list A))) env ->
+    (* GLabelMap.MapsTo fdealloc_one (Axiomatic (FacadeImplementationOfDestructor A)) env -> *)
+    GLabelMap.MapsTo fcons (Axiomatic (FacadeImplementationOfMutation_ADT A' (list A') cons)) env ->
+    PreconditionSet tenv ext ([[[vhead; vhead'; vtest; vlst; vret; vtmp]]]) ->
+    (forall head (s: list A) (s': list A'),
+        {{ [[`vhead <-- head as _]] :: tenv }}
+          facadeBody
+        {{ [[`vhead' <-- f head as _]] :: tenv }} ∪
+        {{ [vret <-- wrap s'] :: [vtest <-- wrap (bool2w false)] :: [vlst <-- wrap s] :: ext }} // env) ->
+    {{ [[`vlst <~~ lst as _]] :: tenv }}
+      (Seq
+         (Call vret falloc nil)
+         (Seq
+            (Fold vhead vtest vlst fpop fempty
+                  (Seq facadeBody
+                       (Call vtmp fcons (vret :: vhead' :: nil))))
+            (Call vtest fdealloc (vlst :: nil))))
+    {{ [[lst as ls]] :: [[`vret <-- (revmap f ls) ++ base as _]] :: tenv }} ∪ {{ ext }} // env.
+Proof.
+  intros.
+  loop_t.
+
+  eapply (CompileCallFacadeImplementationOfConstructor (A := list A') (adt := base)); loop_t.
+
+  rewrite TelEq_swap;
+    eapply CompileCallEmpty_spec; loop_t.
+
+  2:eapply (CompileCallFacadeImplementationOfDestructor (A := list A)); loop_t.
+
+  loop_unify_with_nil_t.
+  rewrite (TelEq_swap _ NTNone).
+
+  apply miniChomp'; loop_t.
+
+  clear dependent falloc;
+  generalize dependent lst;
+    generalize dependent base;
+    induction vv; loop_t.
+
+  rewrite TelEq_swap.
+
+  apply CompileWhileFalse_Loop; loop_t.
+
+  eapply CompileWhileTrue; loop_t.
+
+  apply generalized (CompileCallPop (A := A)); loop_t.
+
+  move_to_front vlst; apply ProgOk_Chomp_Some; loop_t.
+  move_to_front vtest; apply ProgOk_Chomp_Some; loop_t.
+  move_to_front vret; apply ProgOk_Chomp_Some; loop_t.
+  computes_to_inv; subst; defunctionalize_evar; eauto.
+
+  move_to_front vhead'.
+  move_to_front vret.
+  apply CompileCallFacadeImplementationOfMutation_ADT; try compile_do_side_conditions.
+
+  move_to_front vlst.
+  apply CompileCallEmpty_spec; loop_t.
+
+  rewrite CompileMap_helper.
+  loop_t.
+Qed.
+
+Lemma CompileMap_ADT_strong :
+  forall {av A A'} `{FacadeWrapper av (list A)} `{FacadeWrapper av (list A')} `{FacadeWrapper av A} `{FacadeWrapper av A'}
+    (lst: Comp (list A)) vhead vhead' vtest vlst vret vtmp fpop fempty falloc fdealloc fcons facadeBody facadeCoda env (ext: StringMap.t (Value av)) tenv tenv' (f: A -> A'),
+    GLabelMap.MapsTo fpop (Axiomatic (List_pop A)) env ->
+    GLabelMap.MapsTo fempty (Axiomatic (List_empty A)) env ->
+    GLabelMap.MapsTo falloc (Axiomatic (FacadeImplementationOfConstructor (list A') nil)) env ->
+    GLabelMap.MapsTo fdealloc (Axiomatic (FacadeImplementationOfDestructor (list A))) env ->
+    GLabelMap.MapsTo fcons (Axiomatic (FacadeImplementationOfMutation_ADT A' (list A') cons)) env ->
+    (* GLabelMap.MapsTo fdealloc_one (Axiomatic (FacadeImplementationOfDestructor A)) env -> *)
+    PreconditionSet tenv ext [[[vhead; vhead'; vtest; vlst; vret; vtmp]]] ->
+    {{ [[lst as ls]] :: [[`vret <-- (revmap f ls) as _]] :: tenv }}
+      facadeCoda
+    {{ [[lst as ls]] :: [[`vret <-- (revmap f ls) as _]] :: tenv' }} ∪ {{ ext }} // env ->
+    (forall head (s: list A) (s': list A'),
+        {{ [[`vhead <-- head as _]] :: tenv }}
+          facadeBody
+        {{ [[`vhead' <-- f head as _]] :: tenv }} ∪
+        {{ [vret <-- wrap s'] :: [vtest <-- wrap (bool2w false)] :: [vlst <-- wrap s] :: ext }} // env) ->
+    {{ [[`vlst <~~ lst as _]] :: tenv }}
+      (Seq
+         (Seq
+            (Call vret falloc nil)
+            (Seq
+               (Fold vhead vtest vlst fpop fempty
+                     (Seq facadeBody
+                          (Call vtmp fcons (vret :: vhead' :: nil))))
+               (Call vtest fdealloc (vlst :: nil))))
+          facadeCoda)
+    {{ [[lst as ls]] :: [[`vret <-- (revmap f ls) as _]] :: tenv' }} ∪ {{ ext }} // env.
+Proof.
+  intros; hoare.
+  setoid_rewrite (app_nil_end (revmap f _)).
+  apply CompileMap_ADT; eauto.
+Qed.
+
+Lemma CompileMap_SCA:
+  forall {av A} `{FacadeWrapper av (list A)} `{FacadeWrapper av (list W)} `{FacadeWrapper av A}
+    (base: list W) (lst: list A) vhead vhead' vtest vlst vret vtmp fpop fempty falloc fdealloc fcons facadeBody env (ext: StringMap.t (Value av)) (tenv: Telescope av) (f: A -> W),
+    GLabelMap.MapsTo fpop (Axiomatic (List_pop A)) env ->
+    GLabelMap.MapsTo fempty (Axiomatic (List_empty A)) env ->
+    GLabelMap.MapsTo falloc (Axiomatic (FacadeImplementationOfConstructor (list W) base)) env ->
+    GLabelMap.MapsTo fdealloc (Axiomatic (FacadeImplementationOfDestructor (list A))) env ->
+    (* GLabelMap.MapsTo fdealloc_one (Axiomatic (FacadeImplementationOfDestructor A)) env -> *)
+    GLabelMap.MapsTo fcons (Axiomatic (FacadeImplementationOfMutation_SCA (list W) cons)) env ->
+    PreconditionSet tenv ext ([[[vhead; vhead'; vtest; vlst; vret; vtmp]]]) ->
+    (forall head (s: list A) (s': list W),
+        {{ [[`vhead <-- head as _]] :: tenv }}
+          facadeBody
+        {{ [[`vhead' <-- f head as _]] :: tenv }} ∪
+        {{ [vret <-- wrap s'] :: [vtest <-- wrap (bool2w false)] :: [vlst <-- wrap s] :: ext }} // env) ->
+    {{ [[`vlst <-- lst as _]] :: tenv }}
+      (Seq
+         (Call vret falloc nil)
+         (Seq
+            (Fold vhead vtest vlst fpop fempty
+                  (Seq facadeBody
+                       (Call vtmp fcons (vret :: vhead' :: nil))))
+            (Call vtest fdealloc (vlst :: nil))))
+    {{ [[`vret <-- (revmap f lst) ++ base as _]] :: tenv }} ∪ {{ ext }} // env.
+Proof.
+  intros.
+  loop_t.
+
+  eapply (CompileCallFacadeImplementationOfConstructor (A := list W) (adt := base)); loop_t.
+
+  rewrite TelEq_swap;
+    eapply CompileCallEmpty_spec; loop_t.
+
+  2:eapply (CompileCallFacadeImplementationOfDestructor (A := list A)); loop_t.
+
+  loop_unify_with_nil_t.
+  loop_t.
+
+  clear dependent falloc;
+    generalize dependent base;
+    induction lst; loop_t.
+
+  rewrite TelEq_swap.
+
+  apply CompileWhileFalse_Loop; loop_t.
+
+  eapply CompileWhileTrue; loop_t.
+
+  apply generalized (CompileCallPop (A := A)); loop_t.
+
+  move_to_front vlst; apply ProgOk_Chomp_Some; loop_t.
+  move_to_front vtest; apply ProgOk_Chomp_Some; loop_t.
+  move_to_front vret; apply ProgOk_Chomp_Some; loop_t.
+  computes_to_inv; subst; defunctionalize_evar; eauto.
+
+  move_to_front vhead'.
+  move_to_front vret.
+  apply CompileCallFacadeImplementationOfMutation_SCA; try compile_do_side_conditions.
+
+  move_to_front vlst.
+  apply CompileCallEmpty_spec; loop_t.
+
+  rewrite CompileMap_helper.
+  loop_t.
+Qed.
+
+Lemma CompileMap_SCA_strong :
+  forall {av A} `{FacadeWrapper av (list A)} `{FacadeWrapper av (list W)} `{FacadeWrapper av A}
+    (lst: list A) vhead vhead' vtest vlst vret vtmp fpop fempty falloc fdealloc fcons facadeBody facadeCoda env (ext: StringMap.t (Value av)) tenv tenv' (f: A -> W),
+    GLabelMap.MapsTo fpop (Axiomatic (List_pop A)) env ->
+    GLabelMap.MapsTo fempty (Axiomatic (List_empty A)) env ->
+    GLabelMap.MapsTo falloc (Axiomatic (FacadeImplementationOfConstructor (list W) nil)) env ->
+    GLabelMap.MapsTo fdealloc (Axiomatic (FacadeImplementationOfDestructor (list A))) env ->
+    GLabelMap.MapsTo fcons (Axiomatic (FacadeImplementationOfMutation_SCA (list W) cons)) env ->
+    (* GLabelMap.MapsTo fdealloc_one (Axiomatic (FacadeImplementationOfDestructor A)) env -> *)
+    PreconditionSet tenv ext [[[vhead; vhead'; vtest; vlst; vret; vtmp]]] ->
+    {{ [[`vret <-- (revmap f lst) as _]] :: tenv }}
+      facadeCoda
+    {{ [[`vret <-- (revmap f lst) as _]] :: tenv' }} ∪ {{ ext }} // env ->
+    (forall head (s: list A) (s': list W),
+        {{ [[`vhead <-- head as _]] :: tenv }}
+          facadeBody
+        {{ [[`vhead' <-- f head as _]] :: tenv }} ∪
+        {{ [vret <-- wrap s'] :: [vtest <-- wrap (bool2w false)] :: [vlst <-- wrap s] :: ext }} // env) ->
+    {{ [[`vlst <-- lst as _]] :: tenv }}
+      (Seq
+         (Seq
+            (Call vret falloc nil)
+            (Seq
+               (Fold vhead vtest vlst fpop fempty
+                     (Seq facadeBody
+                          (Call vtmp fcons (vret :: vhead' :: nil))))
+               (Call vtest fdealloc (vlst :: nil))))
+          facadeCoda)
+    {{ [[`vret <-- (revmap f lst) as _]] :: tenv' }} ∪ {{ ext }} // env.
+Proof.
+  intros; hoare.
+  setoid_rewrite (app_nil_end (revmap f _)).
+  apply CompileMap_SCA; eauto.
+Qed.
+
 Lemma SameValues_Fiat_Bind_TelEq_Pair :
   forall {av A1 A2 B} key compA compB tail ext,
     TelEq ext
@@ -314,82 +468,130 @@ Proof.
          end.
 Qed.
 
-(* Example other_test_with_adt'''' A: *)
-(*   sigT (fun prog => forall (searchTerm: TSearchTerm) (init: TAcc), *)
-(*             {{ [[`"search" <-- searchTerm as _]] :: [[`"init" <-- init as _]] :: (@Nil av) }} *)
-(*               prog *)
-(*             {{ [[`"ret" <~~  ( seq <- {s: (A * list W) | True }; *)
-(*                              ret (snd seq)) as _]] :: (@Nil av) }} ∪ {{ StringMap.empty (Value av) }} // MyEnvListsB). *)
-(* Proof. *)
-(*   Unset Ltac Debug. *)
-(*   econstructor; intros. *)
-
-(*   rewrite SameValues_Fiat_Bind_TelEq_Pair. *)
-(*   simpl. *)
-
-
 Require Import Fiat.QueryStructure.Implementation.DataStructures.BagADT.QueryStructureImplementation Fiat.QueryStructure.Automation.Common Fiat.QueryStructure.Specification.Representation.Schema.
 Require Import Coq.Vectors.Fin.
 Print PartialSchedulerImpl.
 
-Definition Type1 := IndexedQueryStructure 
+Definition Type1 := IndexedQueryStructure
                      (QueryStructureSchema.QueryStructureSchemaRaw SchedulerSchema)
-                     (@icons3 _ 
-                              (fun sch : RawHeading => SearchUpdateTerms sch) heading 0 
-                              (VectorDef.nil RawHeading) SearchUpdateTerm 
+                     (@icons3 _
+                              (fun sch : RawHeading => SearchUpdateTerms sch) heading 0
+                              (VectorDef.nil RawHeading) SearchUpdateTerm
                               (@inil3 _ (fun sch : RawHeading => SearchUpdateTerms sch))).
 
 Definition Type2 := (Type1 * list (Domain heading (@FS 2 (@FS 1 (@F1 0)))))%type.
 
 Definition MethodOfInterest := fun (r_n : Type1) (d : W) =>
-                                (a <- @CallBagMethod 
+                                (a <- @CallBagMethod
                                    (QueryStructureSchema.QueryStructureSchemaRaw SchedulerSchema)
-                                        (@icons3 _ 
-                                           (fun sch : RawHeading => SearchUpdateTerms sch) heading 0 
-                                           (VectorDef.nil RawHeading) SearchUpdateTerm 
-                                           (@inil3 _ (fun sch : RawHeading => SearchUpdateTerms sch))) 
+                                        (@icons3 _
+                                           (fun sch : RawHeading => SearchUpdateTerms sch) heading 0
+                                           (VectorDef.nil RawHeading) SearchUpdateTerm
+                                           (@inil3 _ (fun sch : RawHeading => SearchUpdateTerms sch)))
                                         (@F1 0)
                                         (@BagFind heading
-                                           (@ilist3_hd RawSchema 
+                                           (@ilist3_hd RawSchema
                                               (fun ns : RawSchema => SearchUpdateTerms (rawSchemaHeading ns)) 1
                                               (Vector.cons RawSchema
                                                  {|
                                                  rawSchemaHeading := heading;
                                                  attrConstraints := @None (@RawTuple heading -> Prop);
-                                                 tupleConstraints := @Some 
-                                                  (@RawTuple heading -> @RawTuple heading -> Prop) 
-                                                  (@FunctionalDependency_P heading [@FS 2 (@FS 1 (@F1 0)); @FS 2 (@F1 1)] [@F1 2]) |} 0 
+                                                 tupleConstraints := @Some
+                                                  (@RawTuple heading -> @RawTuple heading -> Prop)
+                                                  (@FunctionalDependency_P heading [@FS 2 (@FS 1 (@F1 0)); @FS 2 (@F1 1)] [@F1 2]) |} 0
                                                  (Vector.nil RawSchema))
-                                              (@icons3 _ 
-                                                 (fun sch : RawHeading => SearchUpdateTerms sch) heading 0 
-                                                 (VectorDef.nil RawHeading) SearchUpdateTerm 
+                                              (@icons3 _
+                                                 (fun sch : RawHeading => SearchUpdateTerms sch) heading 0
+                                                 (VectorDef.nil RawHeading) SearchUpdateTerm
                                                  (@inil3 _ (fun sch : RawHeading => SearchUpdateTerms sch))))) r_n
                                         (@Some W d, (@None (Domain heading (@FS 2 (@F1 1))), fun _ : @RawTuple heading => true));
                                  ret
                                    (r_n,
-                                   @map (@RawTuple heading) 
+                                   @map (@RawTuple heading)
                                      (Domain heading (@FS 2 (@FS 1 (@F1 0))))
                                      (fun x : @RawTuple heading =>
                                       @GetAttributeRaw heading
-                                        (@ilist2.ilist2_hd RawHeading 
-                                           (@RawTuple) 1 
+                                        (@ilist2.ilist2_hd RawHeading
+                                           (@RawTuple) 1
                                            (VectorDef.cons RawHeading heading 0 (VectorDef.nil RawHeading))
                                            (@ilist2.icons2 RawHeading (@RawTuple) heading 0 (VectorDef.nil RawHeading) x (@ilist2.inil2 RawHeading (@RawTuple))))
-                                        (@FS 2 (@FS 1 (@F1 0)))) 
+                                        (@FS 2 (@FS 1 (@F1 0))))
                                      (@snd (@IndexedEnsembles.IndexedEnsemble (@RawTuple heading)) (list (@RawTuple heading)) a)))%comp : Comp Type2.
 
-Definition av' := (list W + Type1 + Type2)%type.
-
-Definition MyEnvListsC : Env av' :=
-  (GLabelMap.add ("std", "rand") (Axiomatic FRandom))
-    ((GLabelMap.add ("list", "nil") (Axiomatic (FacadeImplementationOfConstructor (@nil W))))
-       ((GLabelMap.add ("list", "push!") (Axiomatic (FacadeImplementationOfMutation (@cons W))))
-          ((GLabelMap.add ("list", "pop!") (Axiomatic List_pop))
-             ((GLabelMap.add ("list", "delete!") (Axiomatic (FacadeImplementationOfDestructor (A := list W))))
-                ((GLabelMap.add ("list", "empty?") (Axiomatic List_empty))
-                   (GLabelMap.empty (FuncSpec _))))))).
+Definition av' := (list W + Type1 + Type2 + (@IndexedEnsembles.IndexedEnsemble
+                                              (@RawTuple heading)) + (list (@RawTuple heading)) + (@RawTuple heading))%type.
 
 Check MethodOfInterest.
+
+(* Notation "'BIND' !! A !! B !! C" := (@Bind A B C) (at level 1). *)
+(* Notation "x { A } <- y ; z" := (Bind y (fun x: A => z)) (at level 1). *)
+
+Lemma ProgOk_Transitivity_Name_Pair :
+  forall {av A1 A2} `{FacadeWrapper av A1} `{FacadeWrapper av A2} {ext env}
+    vfst vsnd tenv tenv' (pair: Comp (A1 * A2)) prog d1 d2,
+    {{ tenv }}
+      prog
+    {{ [[pair as p]] :: [[`vfst <-- fst p as p1]] :: [[`vsnd <-- snd p as p2]] :: tenv' p1 p2 }} ∪ {{ext}} // env ->
+    {{ [[pair as p]] :: [[`vfst <-- fst p as p1]] :: [[`vsnd <-- snd p as p2]] :: tenv' p1 p2 }}
+      d1
+    {{ [[pair as p]] :: [[ret (fst p) as p1]] :: [[`vsnd <-- snd p as p2]] :: tenv' p1 p2 }} ∪ {{ext}} // env ->
+    {{ [[pair as p]] :: [[ret (fst p) as p1]] :: [[`vsnd <-- snd p as p2]] :: tenv' p1 p2 }}
+      d2
+    {{ [[pair as p]] :: [[ret (fst p) as p1]] :: [[ret (snd p) as p2]] :: tenv' p1 p2 }} ∪ {{ext}} // env ->
+    {{ tenv }}
+      Seq prog (Seq d1 d2)
+    {{ [[pair as p]] :: [[ret (fst p) as p1]] :: [[ret (snd p) as p2]] :: tenv' p1 p2 }} ∪ {{ext}} // env.
+Proof.
+  repeat hoare.
+Qed.
+
+About List_pop.
+
+Lemma CompileDeallocADT_discretely : (* TODO create a specialized version that hardcodes the deallocation call *)
+  forall {av A} {env ext} (k: NameTag av A) comp tenv tenv' prog dealloc,
+    {{ [[k <~~ comp as kk]] :: tenv kk }}
+      prog
+      {{ [[k <~~ comp as kk]] :: tenv' kk }} ∪ {{ext}} // env ->
+    {{ [[k <~~ comp as kk]] :: tenv' kk }}
+      dealloc
+      {{ [[comp as kk]] :: tenv' kk }} ∪ {{ext}} // env ->
+    {{ [[k <~~ comp as kk]] :: tenv kk }}
+      (Seq prog dealloc)
+      {{ [[comp as kk]] :: tenv' kk }} ∪ {{ext}} // env.
+Proof.
+  repeat hoare.
+Qed.
+
+Lemma CompileDeallocADT_discretely' : (* TODO create a specialized version that hardcodes the deallocation call *)
+  forall {av A} {env ext} (k: NameTag av A) v tenv tenv' prog dealloc,
+    {{ [[k <-- v as _]] :: tenv }}
+      prog
+    {{ [[k <-- v as _]] :: tenv' }} ∪ {{ext}} // env ->
+    {{ [[k <-- v as _]] :: tenv' }}
+      dealloc
+    {{ tenv' }} ∪ {{ext}} // env ->
+    {{ [[k <-- v as _]] :: tenv }}
+      (Seq prog dealloc)
+    {{ tenv' }} ∪ {{ext}} // env.
+Proof.
+  repeat hoare.
+Qed.
+
+Definition MyEnvListsC : Env av' :=
+  (GLabelMap.empty (FuncSpec _))
+    ### ("std", "rand") ->> (Axiomatic FRandom)
+    ### ("listW", "nil") ->> (Axiomatic (FacadeImplementationOfConstructor (list W) nil))
+    ### ("listW", "push!") ->> (Axiomatic (FacadeImplementationOfMutation_SCA (list W) cons))
+    ### ("listW", "pop!") ->> (Axiomatic (List_pop W))
+    ### ("listW", "delete!") ->> (Axiomatic (FacadeImplementationOfDestructor (list W)))
+    ### ("listW", "empty?") ->> (Axiomatic (List_empty W))
+    ### ("listT", "nil") ->> (Axiomatic (FacadeImplementationOfConstructor (list (@RawTuple heading)) nil))
+    ### ("listT", "push!") ->> (Axiomatic (FacadeImplementationOfMutation_ADT _ (list (@RawTuple heading)) cons))
+    ### ("listT", "pop!") ->> (Axiomatic (List_pop (@RawTuple heading)))
+    ### ("listT", "delete!") ->> (Axiomatic (FacadeImplementationOfDestructor (list (@RawTuple heading))))
+    ### ("listT", "empty?") ->> (Axiomatic (List_empty (@RawTuple heading)))
+    ### ("IndexedEnsemble", "delete!") ->> (Axiomatic (FacadeImplementationOfDestructor IndexedEnsembles.IndexedEnsemble))
+    ### ("RawTuple", "delete!") ->> (Axiomatic (FacadeImplementationOfDestructor (@RawTuple heading))).
 
 Example compile :
   sigT (fun prog => forall (r_n : Type1) (d : W),
@@ -400,108 +602,92 @@ Proof.
   eexists; intros.
   unfold MethodOfInterest.
 
-  (* Notation "'BIND' !! A !! B !! C" := (@Bind A B C) (at level 1). *)
-  (* Notation "x { A } <- y ; z" := (Bind y (fun x: A => z)) (at level 1). *)
-  rewrite SameValues_Fiat_Bind_TelEq_Pair.
-  setoid_rewrite Propagate_anonymous_ret at 3; simpl.
+  rewrite SameValues_Fiat_Bind_TelEq.
+  setoid_rewrite Propagate_anonymous_ret; simpl.
 
-  Eval simpl in (@CallBagMethod (QueryStructureSchema.QueryStructureSchemaRaw SchedulerSchema)
-           (@icons3 RawHeading (fun sch : RawHeading => SearchUpdateTerms sch) heading O 
-              (VectorDef.nil RawHeading) SearchUpdateTerm 
-              (@inil3 RawHeading (fun sch : RawHeading => SearchUpdateTerms sch))) 
-           (@F1 O)
-           (@BagFind heading
-              (@ilist3_hd RawSchema (fun ns : RawSchema => SearchUpdateTerms (rawSchemaHeading ns)) 
-                 (S O)
-                 (Vector.cons RawSchema
-                    (Build_RawSchema heading (@None (@RawTuple heading -> Prop))
-                       (@Some (@RawTuple heading -> @RawTuple heading -> Prop)
-                          (@FunctionalDependency_P heading
-                             (@cons (t (S (S (S O)))) 
-                                (@FS (S (S O)) (@FS (S O) (@F1 O)))
-                                (@cons (t (S (S (S O)))) (@FS (S (S O)) (@F1 (S O))) (@nil (t (S (S (S O)))))))
-                             (@cons (t (S (S (S O)))) (@F1 (S (S O))) (@nil (t (S (S (S O))))))))) O 
-                    (Vector.nil RawSchema))
-                 (@icons3 RawHeading (fun sch : RawHeading => SearchUpdateTerms sch) heading O 
-                    (VectorDef.nil RawHeading) SearchUpdateTerm 
-                    (@inil3 RawHeading (fun sch : RawHeading => SearchUpdateTerms sch))))) r_n
-           (@pair (option W) (prod (option (Domain heading (@FS (S (S O)) (@F1 (S O))))) (@RawTuple heading -> bool)) 
-              (@Some W d)
-              (@pair (option (Domain heading (@FS (S (S O)) (@F1 (S O))))) 
-                 (@RawTuple heading -> bool) (@None (Domain heading (@FS (S (S O)) (@F1 (S O))))) 
-                 (fun _ : @RawTuple heading => true)))).
-
-  Eval simpl in ((fix methodType' (rep : Type) (dom : list Type) (cod : option Type) {struct dom} : 
-        Type :=
-          match dom with
-          | nil => match cod with
-                  | Some cod' => Comp (rep * cod')
-                  | None => Comp rep
-                  end
-          | d :: dom' => d -> methodType' rep dom' cod
-          end)
-         (Core.Rep
-            (BagADT.BagSpec (BagMatchSearchTerm (ith3 (icons3 SearchUpdateTerm inil3) F1))
-               (BagApplyUpdateTerm (ith3 (icons3 SearchUpdateTerm inil3) F1)))) 
-         []
-         (snd
-            (ADTSig.MethodDomCod
-               (BuildADTSig.DecADTSig
-                  (BagADT.BagSig RawTuple (BagSearchTermType (ith3 (icons3 SearchUpdateTerm inil3) F1))
-                     (BagUpdateTermType (ith3 (icons3 SearchUpdateTerm inil3) F1)))) BagFind))).
-
-  
-  eapply ProgOk_Transitivity_Cons; repeat compile_step.
-  Focus 2. eapply ProgOk_Transitivity_Name' with "fst"; repeat compile_step.
-  Focus 2. eapply ProgOk_Transitivity_Name' with "snd"; repeat compile_step.
-  Focus 2. 
-
-
-  
-  simpl.
-  eapply ProgOk_Transitivity_Cons.
-
-
-
-  
-  f_equal.
-  unfold Type2.
-  compute.
-  specialize (H (@NTSome _ _ "ret" (@WrapInstance av' Type2 (@FacadeWrapper_Right (sum (list W) Type1) Type2 Type2 (@FacadeWrapper_Self Type2))))).
-
-  
+  move_to_front "r_n".
   compile_step.
-  
-  Eval compute in (Core.Rep
-          (BagADT.BagSpec (BagMatchSearchTerm (ith3 (icons3 SearchUpdateTerm inil3) F1))
-             (BagApplyUpdateTerm (ith3 (icons3 SearchUpdateTerm inil3) F1)))).
-
-  Set Printing Implicit.
-  Unset Printing Notations.
-  
-  Eval compute in (CallBagMethod (qs_schema := QueryStructureSchema.QueryStructureSchemaRaw SchedulerSchema) F1 BagFind r_n (Some d, (None, fun _ : RawTuple => true))).
-  Eval compute in ((fix methodType' (rep : Type) (dom : list Type) (cod : option Type) {struct dom} : 
-        Type :=
-          match dom with
-          | nil => match cod with
-                  | Some cod' => Comp (rep * cod')
-                  | None => Comp rep
-                  end
-          | d :: dom' => d -> methodType' rep dom' cod
-          end)
-         (Core.Rep
-            (BagADT.BagSpec (BagMatchSearchTerm (ith3 (icons3 SearchUpdateTerm inil3) F1))
-               (BagApplyUpdateTerm (ith3 (icons3 SearchUpdateTerm inil3) F1)))) 
-         []
-         (snd
-            (ADTSig.MethodDomCod
-               (BuildADTSig.DecADTSig
-                  (BagADT.BagSig RawTuple (BagSearchTermType (ith3 (icons3 SearchUpdateTerm inil3) F1))
-                     (BagUpdateTermType (ith3 (icons3 SearchUpdateTerm inil3) F1)))) BagFind))).
   compile_step.
-  forall ,
-    
+  compile_step.
 
+  Ltac compile_CallBagFind :=
+    match_ProgOk
+      ltac:(fun prog pre post ext env =>
+              match constr:(pre, post) with
+              | (Cons (NTSome ?kd) (ret ?d) ?tenv,
+                 Cons NTNone (CallBagMethod ?id BagFind ?v (Some ?d, ?r)) ?tenv') =>
+                let vfst := gensym "fst" in
+                let vsnd := gensym "snd" in
+                let vtmp := gensym "tmp" in
+                match post with
+                | Cons NTNone ?v _ =>
+                  eapply CompileSeq with ([[v as vv]]
+                                            :: [[`vfst <-- fst vv as f]]
+                                            :: [[`vsnd <-- snd vv as s]]
+                                            :: [[ret d as dd]]
+                                            :: (tenv dd));
+                    [ match_ProgOk
+                        ltac:(fun prog' _ _ _ _ =>
+                                unify prog' (Call (DummyArgument vtmp) ("ext", "BagFind")
+                                                  (vfst :: vsnd :: "r_n" :: kd :: nil))) (* FIXME *) | ]
+                end
+              end).
+
+  compile_CallBagFind.
+  admit.
+
+  apply ProgOk_Chomp_None.
+  compile_step.
+
+  apply CompileDeallocADT_discretely'.
+  compile_step.
+  compile_step.
+
+  setoid_rewrite Propagate_anonymous_ret.
+
+  match goal with
+  | [  |- appcontext[@map ?a ?b] ] => replace (@map a b) with (@revmap a b) by admit
+  end.
+
+  let vhead := gensym "head" in
+  let vhead' := gensym "head'" in
+  let vtest := gensym "test" in
+  let vtmp := gensym "tmp" in
+  apply (CompileMap_SCA_strong (snd v0) (vhead := vhead) (vhead' := vhead') (vtest := vtest) (vtmp := DummyArgument vtmp)); try compile_do_side_conditions.
+
+  compile_step.
+  compile_step.
+  compile_step.
+
+  Definition FinToWord {N: nat} (n: Fin.t N) :=
+    Word.natToWord 32 (proj1_sig (Fin.to_nat n)).
+
+  Definition FitsInW {N: nat} (n: Fin.t N) :=
+    Word.wordToNat (FinToWord n) = proj1_sig (Fin.to_nat n).
+
+  assert (FitsInW (@FS 2 (@FS 1 (@F1 0)))) by reflexivity.
+
+  compile_do_use_transitivity_to_handle_head_separately.
+
+  apply CompileSeq with ([[`"index" <-- FinToWord (@FS 2 (@FS 1 (@F1 0))) as _]] :: [[ ` "head" <-- head as _]] :: Nil).
+
+  compile_step.                 (* FIXME shouldn't extend SCA lifespan *)
+  apply CompileSkip. (* FIXME fast-track compile_step this to just apply CompileSkip *)
+  instantiate (1 := Call "head'" ("ext", "GetAttribute") ("head" :: "index" :: nil)).
+  admit.
+
+  compile_step.
+  compile_step.
+  compile_step.
+  let tmp := gensym "tmp" in     (* FIXME prove  deallocation lemma specific to the ret case. *)
+  apply (CompileCallFacadeImplementationOfDestructor (vtmp := DummyArgument tmp)); try compile_do_side_conditions.
+
+  let tmp := gensym "tmp" in     (* FIXME prove  deallocation lemma specific to the ret case. *)
+  apply (CompileCallFacadeImplementationOfDestructor (vtmp := DummyArgument tmp)); try compile_do_side_conditions.
+Defined.
+
+Opaque DummyArgument.
+Eval compute in (extract_facade compile).
 
 Example other_test_with_adt'' :
     sigT (fun prog => forall seq seq', {{ [[`"arg1" <-- seq as _ ]] :: [[`"arg2" <-- seq' as _]] :: Nil }}
@@ -530,7 +716,7 @@ Proof.
   compile_step.
   compile_step.
   compile_step.
-  
+
 
   compile_step.
   Fail fail.
@@ -558,4 +744,17 @@ Abort.
   Proof.
     SameValues_Facade_t.
   Qed.
- 
+
+  
+(* Example other_test_with_adt'''' A: *)
+(*   sigT (fun prog => forall (searchTerm: TSearchTerm) (init: TAcc), *)
+(*             {{ [[`"search" <-- searchTerm as _]] :: [[`"init" <-- init as _]] :: (@Nil av) }} *)
+(*               prog *)
+(*             {{ [[`"ret" <~~  ( seq <- {s: (A * list W) | True }; *)
+(*                              ret (snd seq)) as _]] :: (@Nil av) }} ∪ {{ StringMap.empty (Value av) }} // MyEnvListsB). *)
+(* Proof. *)
+(*   Unset Ltac Debug. *)
+(*   econstructor; intros. *)
+
+(*   rewrite SameValues_Fiat_Bind_TelEq_Pair. *)
+(*   simpl. *)
